Prove the interesting PEG theorems.
Importantly, that well-formed grammars (those without left recursion)
always terminate on input strings (either rejecting or accepting
them).

examples/parsing/pegScript.sml
@@ -23,80 +23,409 @@ val _ = Hol_datatype `pegsym =
 `
 
 val _ = Hol_datatype`
-  peg = <| start : 'b inf ; rules : 'b inf |-> ('a,'b,'c,'e) pegsym ;
+  peg = <| start : ('a,'b,'c,'e) pegsym ;
+           rules : 'b inf |-> ('a,'b,'c,'e) pegsym ;
            cf : 'e -> 'a tok |>
 `
 
 val (peg_eval_rules, peg_eval_ind, peg_eval_cases) = Hol_reln`
-  (∀s c. peg_eval G (empty c, s) (SOME(s, c))) ∧
+  (∀s c. peg_eval G (s, empty c) (SOME(s, c))) ∧
   (∀n r s f.
-       n ∈ FDOM G.rules ∧ peg_eval G (G.rules ' n, s) (SOME(r,c)) ⇒
-       peg_eval G (nt n f, s) (SOME(r, f c))) ∧
-  (∀h t f. peg_eval G (any f, h::t) (SOME (t, f (G.cf h) h))) ∧
-  (∀f. peg_eval G (any f, []) NONE) ∧
-  (∀h e t f. G.cf e = h ⇒ peg_eval G (tok h f, e::t) (SOME(t, f e))) ∧
-  (∀h e t f. G.cf e ≠ h ⇒ peg_eval G (tok h f, e::t) NONE) ∧
-  (∀h f. peg_eval G (tok h f, []) NONE) ∧
-  (∀e s c. peg_eval G (e, s) NONE ⇒ peg_eval G (not e c, s) (SOME(s,c))) ∧
-  (∀e s s' c. peg_eval G (e, s) (SOME s') ⇒ peg_eval G (not e c, s) NONE)  ∧
-  (∀e1 e2 s f. peg_eval G (e1, s) NONE ⇒ peg_eval G (seq e1 e2 f, s) NONE)  ∧
+       n ∈ FDOM G.rules ∧ peg_eval G (s, G.rules ' n) (SOME(r,c)) ⇒
+       peg_eval G (s, nt n f) (SOME(r, f c))) ∧
+  (∀n s f.
+       n ∈ FDOM G.rules ∧ peg_eval G (s, G.rules ' n) NONE ⇒
+       peg_eval G (s, nt n f) NONE) ∧
+  (∀h t f. peg_eval G (h::t, any f) (SOME (t, f (G.cf h) h))) ∧
+  (∀f. peg_eval G ([], any f) NONE) ∧
+  (∀h e t f. G.cf e = h ⇒ peg_eval G (e::t, tok h f) (SOME(t, f e))) ∧
+  (∀h e t f. G.cf e ≠ h ⇒ peg_eval G (e::t, tok h f) NONE) ∧
+  (∀h f. peg_eval G ([], tok h f) NONE) ∧
+  (∀e s c. peg_eval G (s, e) NONE ⇒ peg_eval G (s, not e c) (SOME(s,c))) ∧
+  (∀e s s' c. peg_eval G (s, e) (SOME s') ⇒ peg_eval G (s, not e c) NONE)  ∧
+  (∀e1 e2 s f. peg_eval G (s, e1) NONE ⇒ peg_eval G (s, seq e1 e2 f) NONE)  ∧
   (∀e1 e2 s0 s1 c1 f.
-     peg_eval G (e1, s0) (SOME (s1, c1)) ∧ peg_eval G (e2, s1) NONE ⇒
-     peg_eval G (seq e1 e2 f, s0) NONE) ∧
+     peg_eval G (s0, e1) (SOME (s1, c1)) ∧ peg_eval G (s1, e2) NONE ⇒
+     peg_eval G (s0, seq e1 e2 f) NONE) ∧
   (∀e1 e2 s0 s1 s2 c1 c2 f.
-     peg_eval G (e1, s0) (SOME(s1, c1)) ∧
-     peg_eval G (e2, s1) (SOME(s2, c2)) ⇒
-     peg_eval G (seq e1 e2 f, s0) (SOME(s2, f c1 c2))) ∧
+     peg_eval G (s0, e1) (SOME(s1, c1)) ∧
+     peg_eval G (s1, e2) (SOME(s2, c2)) ⇒
+     peg_eval G (s0, seq e1 e2 f) (SOME(s2, f c1 c2))) ∧
   (∀e1 e2 s f.
-     peg_eval G (e1, s) NONE ∧ peg_eval G (e2, s) NONE ⇒
-     peg_eval G (choice e1 e2 f, s) NONE) ∧
+     peg_eval G (s, e1) NONE ∧ peg_eval G (s, e2) NONE ⇒
+     peg_eval G (s, choice e1 e2 f) NONE) ∧
   (∀e1 e2 s s' f c.
-     peg_eval G (e1, s) (SOME(s',c)) ⇒
-     peg_eval G (choice e1 e2 f, s) (SOME(s', f (INL c)))) ∧
+     peg_eval G (s, e1) (SOME(s',c)) ⇒
+     peg_eval G (s, choice e1 e2 f) (SOME(s', f (INL c)))) ∧
   (∀e1 e2 s s' f c.
-     peg_eval G (e1, s) NONE ∧ peg_eval G (e2, s) (SOME(s',c)) ⇒
-     peg_eval G (choice e1 e2 f, s) (SOME(s',f (INR c))))  ∧
+     peg_eval G (s, e1) NONE ∧ peg_eval G (s, e2) (SOME(s',c)) ⇒
+     peg_eval G (s, choice e1 e2 f) (SOME(s',f (INR c))))  ∧
   (∀e f s s1 list.
-     peg_eval_list G (e, s) (SOME(s1,list)) ⇒
-     peg_eval G (rpt e f, s) (SOME(s1, f list))) ∧
-  (∀e s. peg_eval G (e, s) NONE ⇒ peg_eval_list G (e, s) (SOME(s,[]))) ∧
+     peg_eval_list G (s, e) (s1,list) ⇒
+     peg_eval G (s, rpt e f) (SOME(s1, f list))) ∧
+  (∀e s. peg_eval G (s, e) NONE ⇒ peg_eval_list G (s, e) (s,[])) ∧
   (∀e s0 s1 s2 c cs.
-     peg_eval G (e, s0) (SOME(s1,c)) ∧
-     peg_eval_list G (e, s1) (SOME(s2,cs)) ⇒
-     peg_eval_list G (e, s0) (SOME(s2,c::cs)))
+     peg_eval G (s0, e) (SOME(s1,c)) ∧
+     peg_eval_list G (s1, e) (s2,cs) ⇒
+     peg_eval_list G (s0, e) (s2,c::cs))
 `;
 
+val ind' = theorem "peg_eval_strongind"
+             |> SIMP_RULE (srw_ss()) [pairTheory.FORALL_PROD]
+             |> Q.SPECL [`G`, `\es0 r. P1 (FST es0) (SND es0) r`,
+                         `\es0 sr. P2 (FST es0) (SND es0) (FST sr) (SND sr)`]
+             |> SIMP_RULE (srw_ss()) []
+
+open rich_listTheory
+val peg_eval_suffix0 = prove(
+  ``(∀s0 e sr. peg_eval G (s0,e) sr ⇒ ∀s r. sr = SOME (s,r) ⇒ IS_SUFFIX s0 s) ∧
+    ∀s0 e s rl. peg_eval_list G (s0,e) (s,rl) ⇒ IS_SUFFIX s0 s``,
+  HO_MATCH_MP_TAC ind' THEN SRW_TAC [][IS_SUFFIX_compute, IS_PREFIX_APPEND3,
+                                       IS_PREFIX_REFL] THEN
+  METIS_TAC [IS_PREFIX_TRANS]);
+
+(* Theorem 3.1 *)
+val peg_eval_suffix = save_thm(
+  "peg_eval_suffix",
+  peg_eval_suffix0 |> SIMP_RULE (srw_ss() ++ DNF_ss) [])
+
+(* Theorem 3.2 *)
+val peg_deterministic = store_thm(
+  "peg_deterministic",
+  ``(∀s0 e sr. peg_eval G (s0,e) sr ⇒ ∀sr'. peg_eval G (s0,e) sr' ⇔ sr' = sr) ∧
+    ∀s0 e s rl. peg_eval_list G (s0,e) (s,rl) ⇒
+                ∀srl'. peg_eval_list G (s0,e) srl' ⇔ srl' = (s,rl)``,
+  HO_MATCH_MP_TAC ind' THEN SRW_TAC [][] THEN
+  ONCE_REWRITE_TAC [peg_eval_cases] THEN SRW_TAC [][]);
+
+open lcsymtacs
+(* Lemma 3.3 *)
+val peg_badrpt = store_thm(
+  "peg_badrpt",
+  ``peg_eval G (s0,e) (SOME(s0,r)) ⇒ ∀r. ¬peg_eval G (s0, rpt e f) r``,
+  strip_tac >> simp[Once peg_eval_cases] >> map_every qx_gen_tac [`s1`, `l`] >>
+  disch_then (assume_tac o MATCH_MP (CONJUNCT2 peg_deterministic)) >>
+  `peg_eval_list G (s0,e) (s1,r::l)`
+    by METIS_TAC [last (peg_eval_rules |> SPEC_ALL |> CONJUNCTS)] >>
+  pop_assum mp_tac >> simp[]);
+
+val (peg0_rules, peg0_ind, peg0_cases) = Hol_reln`
+  (∀c. peg0 G (empty c)) ∧
+
+  (* any *)
+  (∀f. peggt0 G (any f)) ∧
+  (∀f. pegfail G (any f)) ∧
+
+  (* tok *)
+  (∀t f. peggt0 G (tok t f)) ∧
+  (∀t f. pegfail G (tok t f)) ∧
+
+  (* rpt *)
+  (∀e f. pegfail G e ⇒ peg0 G (rpt e f)) ∧
+  (∀e f. peggt0 G e ⇒ peggt0 G (rpt e f)) ∧
+
+  (* nt rules *)
+  (∀n f. n ∈ FDOM G.rules ∧ peg0 G (G.rules ' n) ⇒
+         peg0 G (nt n f)) ∧
+  (∀n f. n ∈ FDOM G.rules ∧ peggt0 G (G.rules ' n) ⇒
+         peggt0 G (nt n f)) ∧
+  (∀n f. n ∈ FDOM G.rules ∧ pegfail G (G.rules ' n) ⇒
+         pegfail G (nt n f)) ∧
+
+  (* seq rules *)
+  (∀e1 e2 f. pegfail G e1 ∨ (peg0 G e1 ∧ pegfail G e2) ∨
+             (peggt0 G e1 ∧ pegfail G e2) ⇒
+             pegfail G (seq e1 e2 f)) ∧
+  (∀e1 e2 f. peggt0 G e1 ∧ (peg0 G e2 ∨ peggt0 G e2) ∨
+             (peg0 G e1 ∨ peggt0 G e1) ∧ peggt0 G e2 ⇒
+             peggt0 G (seq e1 e2 f)) ∧
+  (∀e1 e2 f. peg0 G e1 ∧ peg0 G e2 ⇒ peg0 G (seq e1 e2 f)) ∧
+
+  (* choice rules *)
+  (∀e1 e2 f. peg0 G e1 ∨ (pegfail G e1 ∧ peg0 G e2) ⇒
+             peg0 G (choice e1 e2 f)) ∧
+  (∀e1 e2 f. pegfail G e1 ∧ pegfail G e2 ⇒ pegfail G (choice e1 e2 f)) ∧
+  (∀e1 e2 f. peggt0 G e1 ∨ (pegfail G e1 ∧ peggt0 G e2) ⇒
+             peggt0 G (choice e1 e2 f)) ∧
+
+  (* not *)
+  (∀e c. pegfail G e ⇒ peg0 G (not e c)) ∧
+  (∀e c. peg0 G e ∨ peggt0 G e ⇒ pegfail G (not e c))
+`;
+
+val peg_eval_suffix' = store_thm(
+  "peg_eval_suffix'",
+  ``peg_eval G (s0,e) (SOME(s,c)) ⇒
+    s0 = s ∨ IS_SUFFIX s0 s ∧ LENGTH s < LENGTH s0``,
+  strip_tac >> imp_res_tac peg_eval_suffix >> Cases_on `s0 = s` >- simp[] >>
+  fs[IS_SUFFIX_compute] >>
+  imp_res_tac IS_PREFIX_LENGTH >> fs[] >>
+  qsuff_tac `LENGTH s ≠ LENGTH s0` >- (strip_tac >> decide_tac) >>
+  strip_tac >>
+  metis_tac [IS_PREFIX_LENGTH_ANTI, LENGTH_REVERSE, REVERSE_REVERSE]);
+
+val peg_eval_list_suffix' = store_thm(
+  "peg_eval_list_suffix'",
+  ``peg_eval_list G (s0, e) (s,rl) ⇒
+    s0 = s ∨ IS_SUFFIX s0 s ∧ LENGTH s < LENGTH s0``,
+  strip_tac >> imp_res_tac peg_eval_suffix >> Cases_on `s0 = s` >- simp[] >>
+  fs[IS_SUFFIX_compute] >> imp_res_tac IS_PREFIX_LENGTH >> fs[] >>
+  qsuff_tac `LENGTH s ≠ LENGTH s0` >- (strip_tac >> decide_tac) >> strip_tac >>
+  metis_tac [IS_PREFIX_LENGTH_ANTI, LENGTH_REVERSE, REVERSE_REVERSE]);
+
+
+fun rule_match th = FIRST (List.mapPartial (total MATCH_MP_TAC)
+                                           (th |> SPEC_ALL |> CONJUNCTS))
+
+val lemma4_1a0 = prove(
+  ``(∀s0 e r. peg_eval G (s0, e) r ⇒
+              (∀c. r = SOME(s0,c) ⇒ peg0 G e) ∧
+              (r = NONE ⇒ pegfail G e) ∧
+              (∀s c. r = SOME(s,c) ∧ LENGTH s < LENGTH s0 ⇒ peggt0 G e)) ∧
+    (∀s0 e s rl. peg_eval_list G (s0,e) (s,rl) ⇒
+                 (s0 = s ⇒ pegfail G e) ∧
+                 (LENGTH s < LENGTH s0 ⇒ peggt0 G e))``,
+  ho_match_mp_tac ind' >> simp[peg0_rules] >> rpt conj_tac
+  >- (rpt strip_tac >> imp_res_tac peg_eval_suffix' >> fs[peg0_rules])
+  >- (rpt strip_tac >> rule_match peg0_rules >>
+      imp_res_tac peg_eval_suffix' >> fs[] >> rw[] >>
+      full_simp_tac (srw_ss() ++ ARITH_ss) [])
+  >- (rpt strip_tac >> rule_match peg0_rules >>
+      imp_res_tac peg_eval_suffix' >> fs[] >> rw[] >>
+      full_simp_tac (srw_ss() ++ ARITH_ss) []) >>
+  rpt strip_tac
+  >- (first_x_assum match_mp_tac >> rw[] >>
+      imp_res_tac peg_eval_suffix >> fs[IS_SUFFIX_compute] >>
+      imp_res_tac IS_PREFIX_LENGTH >> fs[] >>
+      `LENGTH s = LENGTH s0'` by decide_tac >>
+      metis_tac [IS_PREFIX_LENGTH_ANTI, LENGTH_REVERSE, REVERSE_REVERSE]) >>
+  imp_res_tac peg_eval_suffix' >- rw[] >>
+  imp_res_tac peg_eval_list_suffix' >- rw[] >>
+  asm_simp_tac (srw_ss() ++ ARITH_ss) [])
+
+val lemma4_1a = lemma4_1a0 |> SIMP_RULE (srw_ss() ++ DNF_ss) [AND_IMP_INTRO]
+
+val (wfpeg_rules, wfpeg_ind, wfpeg_cases) = Hol_reln`
+  (∀n f. n ∈ FDOM G.rules ∧ wfpeg G (G.rules ' n) ⇒ wfpeg G (nt n f)) ∧
+  (∀c. wfpeg G (empty c)) ∧
+  (∀f. wfpeg G (any f)) ∧
+  (∀t f. wfpeg G (tok t f)) ∧
+  (∀e c. wfpeg G e ⇒ wfpeg G (not e c)) ∧
+  (∀e1 e2 f. wfpeg G e1 ∧ (peg0 G e1 ⇒ wfpeg G e2) ⇒
+             wfpeg G (seq e1 e2 f)) ∧
+  (∀e1 e2 f. wfpeg G e1 ∧ wfpeg G e2 ⇒ wfpeg G (choice e1 e2 f)) ∧
+  (∀e f. wfpeg G e ∧ ¬peg0 G e ⇒ wfpeg G (rpt e f))
+`
+
+val subexprs_def = Define`
+  (subexprs (any f1) = { any f1 }) ∧
+  (subexprs (empty c) = { empty c }) ∧
+  (subexprs (tok t f2) = { tok t f2 }) ∧
+  (subexprs (nt s f) = { nt s f }) ∧
+  (subexprs (not e c) = not e c INSERT subexprs e) ∧
+  (subexprs (seq e1 e2 f3) = seq e1 e2 f3 INSERT subexprs e1 ∪ subexprs e2) ∧
+  (subexprs (choice e1 e2 f4) =
+    choice e1 e2 f4 INSERT subexprs e1 ∪ subexprs e2) ∧
+  (subexprs (rpt e f5) = rpt e f5 INSERT subexprs e)
+`
+val _ = export_rewrites ["subexprs_def"]
+
+
+val subexprs_included = store_thm(
+  "subexprs_included",
+  ``e ∈ subexprs e``,
+  Induct_on `e` >> srw_tac[][subexprs_def] )
+
+val Gexprs_def = Define`
+  Gexprs G = BIGUNION (IMAGE subexprs (G.start INSERT FRANGE G.rules))
+`
+
+val wfG_def = Define`wfG G ⇔ ∀e. e ∈ Gexprs G ⇒ wfpeg G e`;
+
+val IN_subexprs_TRANS = store_thm(
+  "IN_subexprs_TRANS",
+  ``∀a b c. a ∈ subexprs b ∧ b ∈ subexprs c ⇒ a ∈ subexprs c``,
+  Induct_on `c` >> simp[] >> rpt strip_tac >> fs[] >> metis_tac[]);
+
+val Gexprs_subexprs = store_thm(
+  "Gexprs_subexprs",
+  ``e ∈ Gexprs G ⇒ subexprs e ⊆ Gexprs G``,
+  simp_tac (srw_ss() ++ DNF_ss) [Gexprs_def, pred_setTheory.SUBSET_DEF] >>
+  strip_tac >> metis_tac [IN_subexprs_TRANS]);
+
+val IN_Gexprs_E = store_thm(
+  "IN_Gexprs_E",
+  ``(not e c ∈ Gexprs G ⇒ e ∈ Gexprs G) ∧
+    (seq e1 e2 f ∈ Gexprs G ⇒ e1 ∈ Gexprs G ∧ e2 ∈ Gexprs G) ∧
+    (choice e1 e2 f2 ∈ Gexprs G ⇒ e1 ∈ Gexprs G ∧ e2 ∈ Gexprs G) ∧
+    (rpt e f3 ∈ Gexprs G ⇒ e ∈ Gexprs G)``,
+  rpt strip_tac >> imp_res_tac Gexprs_subexprs >> fs[] >>
+  metis_tac [pred_setTheory.SUBSET_DEF, subexprs_included]);
+
+val pair_CASES = pairTheory.pair_CASES
+val option_CASES = optionTheory.option_nchotomy
+val list_CASES = listTheory.list_CASES
+
+val reducing_peg_eval_makes_list = prove(
+  ``(∀s. LENGTH s < n ⇒ ∃r. peg_eval G (s, e) r) ∧ ¬peg0 G e ∧ LENGTH s0 < n ⇒
+    ∃s' rl. peg_eval_list G (s0,e) (s',rl)``,
+  strip_tac >> completeInduct_on `LENGTH s0` >> rw[] >>
+  full_simp_tac (srw_ss() ++ DNF_ss ++ ARITH_ss) [] >>
+  `peg_eval G (s0,e) NONE ∨ ∃s1 c. peg_eval G (s0,e) (SOME(s1,c))`
+    by metis_tac [pair_CASES, option_CASES]
+  >- metis_tac [peg_eval_rules] >>
+  `s0 ≠ s1` by metis_tac [lemma4_1a] >>
+  `LENGTH s1 < LENGTH s0` by metis_tac [peg_eval_suffix'] >>
+  metis_tac [peg_eval_rules]);
+
+
+val peg_eval_total = prove(
+  ``wfG G ⇒ ∀s e. e ∈ Gexprs G ⇒ ∃r. peg_eval G (s,e) r``,
+  simp[wfG_def] >> strip_tac >> gen_tac >>
+  completeInduct_on `LENGTH s` >>
+  full_simp_tac (srw_ss() ++ DNF_ss) [] >> rpt strip_tac >>
+  `wfpeg G e` by metis_tac[] >>
+  Q.UNDISCH_THEN `e ∈ Gexprs G` mp_tac >>
+  pop_assum mp_tac >> qid_spec_tac `e` >>
+  Induct_on `wfpeg` >> rw[]
+  >- ((* nt *)
+      qsuff_tac `G.rules ' n ∈ Gexprs G`
+      >- metis_tac [peg_eval_rules, option_CASES, pair_CASES] >>
+      asm_simp_tac (srw_ss() ++ DNF_ss) [Gexprs_def, FRANGE_DEF] >>
+      metis_tac [subexprs_included])
+  >- (* empty *) metis_tac [peg_eval_rules]
+  >- (* any *) metis_tac [peg_eval_rules, list_CASES]
+  >- (* tok *) metis_tac [peg_eval_rules, list_CASES]
+  >- (* not *) metis_tac [peg_eval_rules, optionTheory.option_nchotomy,
+                          IN_Gexprs_E]
+  >- ((* seq *) Q.MATCH_ASSUM_ABBREV_TAC `seq e1 e2 f ∈ Gexprs G` >>
+      markerLib.RM_ALL_ABBREVS_TAC >>
+      `e1 ∈ Gexprs G` by imp_res_tac IN_Gexprs_E >>
+      `peg_eval G (s,e1) NONE ∨ ∃s' c. peg_eval G (s,e1) (SOME(s',c))`
+        by metis_tac[option_CASES, pair_CASES]
+      >- metis_tac [peg_eval_rules] >>
+      Cases_on `s' = s`
+      >- (`peg0 G e1` by metis_tac [lemma4_1a] >>
+          `e2 ∈ Gexprs G` by imp_res_tac IN_Gexprs_E >>
+          metis_tac [peg_eval_rules, option_CASES, pair_CASES]) >>
+      `LENGTH s' < LENGTH s` by metis_tac [peg_eval_suffix'] >>
+      `∃r'. peg_eval G (s',e2) r'` by metis_tac [IN_Gexprs_E] >>
+      metis_tac [option_CASES, pair_CASES, peg_eval_rules])
+  >- (* choice *)
+     metis_tac [peg_eval_rules, option_CASES, IN_Gexprs_E, pair_CASES] >>
+  (* rpt *) imp_res_tac IN_Gexprs_E >>
+  `peg_eval G (s, e) NONE ∨ ∃s' c. peg_eval G (s,e) (SOME (s',c))`
+    by metis_tac [option_CASES, pair_CASES]
+  >- (`peg_eval_list G (s,e) (s,[])` by metis_tac [peg_eval_rules] >>
+      metis_tac [peg_eval_rules]) >>
+  `s' ≠ s` by metis_tac [lemma4_1a] >>
+  `LENGTH s' < LENGTH s` by metis_tac [peg_eval_suffix'] >>
+  metis_tac [peg_eval_rules, reducing_peg_eval_makes_list])
+
+
+
+
+
+(*
 val _ = Hol_datatype`ftok = Plus | Times | Number | LParen | RParen`
 
 val _ = Hol_datatype`etok = EPlus | ETimes | ENumber of num | ELParen | ERParen`
 
 val categorise_def = Define`
-  categorise EPlus = Plus ∧
-  categorise ETimes = Times ∧
-  categorise (ENumber n) = Number ∧
-  categorise ELParen = LParen ∧
-  categorise ERParen = RParen
+  categorise EPlus = mkTok Plus ∧
+  categorise ETimes = mkTok Times ∧
+  categorise (ENumber n) = mkTok Number ∧
+  categorise ELParen = mkTok LParen ∧
+  categorise ERParen = mkTok RParen
 `;
 
 local open stringTheory in end
 
-val _ = Hol_datatype `expr = XN of num | XPlus of expr => expr | XTimes of expr => expr`
+val _ = Hol_datatype `
+  expr = XN of num
+       | XPlus of expr => expr
+       | XTimes of expr => expr
+       | XList of expr list`;
 
 val _ = overload_on("mkTok", ``mk_finite_image``)
 
 
+val ty = ty_antiq ``:(ftok, string, expr, etok) pegsym``
 val nrule =
-  ``tok (mkTok Number) (\e. case e of ENumber n => XN n)``
+  ``tok (mkTok Number) (\e. case e of ENumber n => XN n) : ^ty``
 val paren_rule =
   ``seq (tok (mkTok LParen) (K (XN 0)))
         (seq (nt (INL "expr") I) (tok (mkTok RParen) (K (XN 0))) (\a b. a))
-        (\a b. b)``
+        (\a b. b) : ^ty``
+
+val termpair =
+  ``(INL "term" : string inf,
+     choice ^nrule ^paren_rule (\s. case s of INL e => e | INR e => e))``
+
+val factorpair = ``(INL "factor" : string inf,
+                    seq (rpt (seq (nt (INL "term") I)
+                                            (tok (mkTok Times) (K ARB))
+                                            (\a b. a))
+                                       XList)
+                                  (nt (INL "term") I)
+                                  (\a b.
+                                    case a of
+                                      XList (h::t) => FOLDL XTimes h (t ++ [b])
+                                    | _ => b) : ^ty)``
+
+val exprpair = ``(INL "expr" : string inf,
+                  seq (rpt (seq (nt (INL "factor") I)
+                                        (tok (mkTok Plus) (K ARB))
+                                        (\a b. a))
+                                   XList)
+                              (nt (INL "factor") I)
+                              (\a b.
+                                case a of
+                                  XList (h::t) => FOLDL XPlus h (t ++ [b])
+                                | _ => b) : ^ty)``
+
+val rules = ``FEMPTY |+ ^exprpair |+ ^factorpair |+ ^termpair``
+
+val G = ``<| start := INL "expr"; rules := ^rules; cf := categorise |>``
+
+val testexp = ``[ENumber 3; EPlus; ENumber 4; ETimes; ENumber 5]``
+
+val [emptyI,ntI0,anyOKI,anyFAIL,tokOK,tokFAIL1,tokFAIL2,notOK, notFAIL,
+     seqFAIL1, seqFAIL2, seqOK0, choiceFAIL, choiceOK1, choiceOK2,
+     rptOK1, list1, list2] = peg_eval_rules |> SPEC_ALL |> CONJUNCTS
+
+val seqOK = let
+  val th0 = seqOK0 |> SPEC_ALL |> UNDISCH
+  val c = th0 |> concl
+  fun check t = let
+    val (f, args) = strip_comb t
+  in
+    not (null args) andalso is_var f
+  end
+  val fxy = find_term check c
+  val th = REWRITE_RULE [ASSUME (mk_eq(fxy, mk_var("x", type_of fxy)))] th0
+in
+  DISCH_ALL th |> REWRITE_RULE [AND_IMP_INTRO] |> GEN_ALL
+end
+
+val ntI = ntI0 |> SPEC_ALL
+               |> Q.INST [`f` |-> `I`]
+               |> SIMP_RULE (srw_ss()) []
+
+val _ = overload_on ("G", G)
+
+val ok = prove(
+  ``peg_eval ^G (nt ^G.start I,^testexp)
+                (SOME([], XPlus (XN 3) (XTimes (XN 4) (XN 5))))``,
+  SIMP_TAC (srw_ss()) [] THEN
+  MATCH_MP_TAC ntI THEN
+  SIMP_TAC (srw_ss()) [finite_mapTheory.FAPPLY_FUPDATE_THM] THEN
+  MATCH_MP_TAC seqOK THEN SIMP_TAC (srw_ss()) []
+
+  FIRST (List.mapPartial (Lib.total MATCH_MP_TAC) (CONJUNCTS peg_eval_rules))
 
 
-val rules = ``FEMPTY |+ ("term", choice ^nrule ^paren_rule (\s. case s of INL e => e | INR e => e))``
 
 
-
-
-
+*)
 val _ = export_theory()
